DeterminismProof updated.(some explanation with clean codebase added.)

src/DeterminismProof.lean
@@ -21,97 +21,107 @@ def evalExpr (e : Expr) (s : State) : Int :=
   match e with
   | Expr.num n => n
   | Expr.var x => s x
-  | Expr.add e1 e2 => evalExpr e1 s + evalExpr e2 s
+  | Expr.add e1 e2 => evalExpr e1 s + evalExpr e2 s -- this is recursion
   | Expr.lt e1 e2 =>
       if evalExpr e1 s < evalExpr e2 s then 1 else 0
 
-def update (s : State) (x : Var) (v : Int) : State :=
+def update (s : State) (x : Var) (v : Int) : State := -- here the type of y is var because we knew that the output must be state , so as we said before the state := var -> Int , so the update get's {y : var} for updating the current state
   fun y => if y == x then v else s y
 
 inductive BigStep : Stmt -> State -> State -> Prop where
-  | assign : forall x e s,
+  | assign (x : Var) (e : Expr) (s : State) :
       BigStep
-        (Stmt.assign x e)
-        s
-        (update s x (evalExpr e s))
+        (Stmt.assign x e) -- this is the main statement that we note in the definition of BigStep
+        s -- this is the pervious state
+        (update s x (evalExpr e s)) -- this is the next state known as s'(updated in some Var in the consider state and outdate for other depends that var are updated in pervious assignment state or not)
 
-  | seq : forall S1 S2 s smid sout,
-      BigStep S1 s smid ->
-      BigStep S2 smid sout ->
-      BigStep (Stmt.seq S1 S2) s sout
+  | seq (S1 : Stmt) (S2 : Stmt) (s : State) (smid : State) (sout : State) :
+      BigStep S1 s smid -> -- updated state for first Statement
+      BigStep S2 smid sout ->  -- updated state for the second Statement
+      BigStep (Stmt.seq S1 S2) s sout -- this step known as final step that define the whole BigStep institution
 
-  | ifTrue : forall b S1 S2 s sout,
-      evalExpr b s ≠ 0 ->
-      BigStep S1 s sout ->
-      BigStep (Stmt.ifElse b S1 S2) s sout
+  | ifTrue (b : Expr) (S1 : Stmt) (S2 : Stmt) (s : State) (sout : State) :
+      evalExpr b s ≠ 0 -> -- if the condition was validate duo to how we define the lt in evalExpr
+      BigStep S1 s sout -> -- if the condition is provided , process the ifTrue(S1) body Stmt
+      BigStep (Stmt.ifElse b S1 S2) s sout -- so whole structure is if b then S1 else S2 , and from state s get updated to sout
 
   | ifFalse : forall b S1 S2 s sout,
-      evalExpr b s = 0 ->
-      BigStep S2 s sout ->
+      evalExpr b s = 0 -> -- if the condition is not provided
+      BigStep S2 s sout -> -- means process the else body and go from state s to sout(updated state)
       BigStep (Stmt.ifElse b S1 S2) s sout
 
-  | whileF : forall b S s,
+  | whileF (b : Expr) (S : Stmt) (s : State) :
       evalExpr b s = 0 ->
-      BigStep (Stmt.while b S) s s
+      BigStep (Stmt.while b S) s s -- here because the loop condition is not provided , so there is no transformation in logics so no change in states
 
-  | whileT : forall b S s smid sout,
+  | whileT (b : Expr) (S : Stmt) (s : State) (smid : State) (sout : State) :
       evalExpr b s ≠ 0 ->
       BigStep S s smid ->
-      BigStep (Stmt.while b S) smid sout ->
+      BigStep (Stmt.while b S) smid sout -> -- this line and previous line defined the iteration logic of our loop
       BigStep (Stmt.while b S) s sout
 
 theorem determinism :
-    forall {S s s1 s2},
-      BigStep S s s1 -> BigStep S s s2 -> s1 = s2 := by
-  intro S s s1 s2 h1
-  induction h1 generalizing s2 with
+    forall
+      {program : Stmt}
+      {startState : State}
+      {finalState1 : State}
+      {finalState2 : State},
+      BigStep program startState finalState1 ->
+      BigStep program startState finalState2 ->
+      finalState1 = finalState2 := by
+
+  intro program startState finalState1 finalState2 firstRun
+
+  induction firstRun generalizing finalState2 with
 
   | assign x e s =>
-      intro h2
-      cases h2 with
-      | assign x e s =>
+      intro secondRun
+      cases secondRun with
+      | assign x2 e2 s2 =>
           rfl
 
-  | seq S1 S2 s smid sout hFirst1 hSecond1 ihFirst ihSecond =>
-      intro h2
-      cases h2 with
-      | seq S1' S2' s' smid2 sout2 hFirst2 hSecond2 =>
-          have hmid : smid = smid2 := ihFirst hFirst2
-          cases hmid
-          exact ihSecond hSecond2
+  | seq S1 S2 s sMid1 sOut1 firstPartRun1 secondPartRun1 ihFirstPart ihSecondPart =>
+      intro secondRun
+      cases secondRun with
+      | seq S1' S2' s' sMid2 sOut2 firstPartRun2 secondPartRun2 =>
+          have sameMiddleState : sMid1 = sMid2 :=
+            ihFirstPart firstPartRun2
+          cases sameMiddleState
+          exact ihSecondPart secondPartRun2
 
-  | ifTrue b S1 S2 s sout hb hThen ihThen =>
-      intro h2
-      cases h2 with
-      | ifTrue b' S1' S2' s' sout2 hb2 hThen2 =>
-          exact ihThen hThen2
-      | ifFalse b' S1' S2' s' sout2 hb0 hElse2 =>
-          exact False.elim (hb hb0)
+  | ifTrue b S1 S2 s sOut1 conditionIsTrue thenRun1 ihThen =>
+      intro secondRun
+      cases secondRun with
+      | ifTrue b' S1' S2' s' sOut2 conditionIsTrue2 thenRun2 =>
+          exact ihThen thenRun2
+      | ifFalse b' S1' S2' s' sOut2 conditionIsFalse elseRun2 =>
+          exact False.elim (conditionIsTrue conditionIsFalse)
 
-  | ifFalse b S1 S2 s sout hb hElse ihElse =>
-      intro h2
-      cases h2 with
-      | ifTrue b' S1' S2' s' sout2 hbNonZero hThen2 =>
-          exact False.elim (hbNonZero hb)
-      | ifFalse b' S1' S2' s' sout2 hb2 hElse2 =>
-          exact ihElse hElse2
+  | ifFalse b S1 S2 s sOut1 conditionIsFalse elseRun1 ihElse =>
+      intro secondRun
+      cases secondRun with
+      | ifTrue b' S1' S2' s' sOut2 conditionIsTrue thenRun2 =>
+          exact False.elim (conditionIsTrue conditionIsFalse)
+      | ifFalse b' S1' S2' s' sOut2 conditionIsFalse2 elseRun2 =>
+          exact ihElse elseRun2
 
-  | whileF b S s hb =>
-      intro h2
-      cases h2 with
-      | whileF b' S' s' hb2 =>
+  | whileF b S s conditionIsFalse =>
+      intro secondRun
+      cases secondRun with
+      | whileF b' S' s' conditionIsFalse2 =>
           rfl
-      | whileT b' S' s' smid2 sout2 hbNonZero hBody hLoop =>
-          exact False.elim (hbNonZero hb)
+      | whileT b' S' s' sMid2 sOut2 conditionIsTrue bodyRun loopRun =>
+          exact False.elim (conditionIsTrue conditionIsFalse)
 
-  | whileT b S s smid sout hb hBody1 hLoop1 ihBody ihLoop =>
-      intro h2
-      cases h2 with
-      | whileF b' S' s' hb0 =>
-          exact False.elim (hb hb0)
-      | whileT b' S' s' smid2 sout2 hb2 hBody2 hLoop2 =>
-          have hmid : smid = smid2 := ihBody hBody2
-          cases hmid
-          exact ihLoop hLoop2
+  | whileT b S s sMid1 sOut1 conditionIsTrue bodyRun1 loopRun1 ihBody ihLoop =>
+      intro secondRun
+      cases secondRun with
+      | whileF b' S' s' conditionIsFalse =>
+          exact False.elim (conditionIsTrue conditionIsFalse)
+      | whileT b' S' s' sMid2 sOut2 conditionIsTrue2 bodyRun2 loopRun2 =>
+          have sameMiddleState : sMid1 = sMid2 :=
+            ihBody bodyRun2
+          cases sameMiddleState
+          exact ihLoop loopRun2
 
 end DeterminismProof
